coq/JsCorrectness.v
@@ -1,3 +1,5 @@
+(* (* Temporary *)
+
 Set Implicit Arguments.
 Require Import Shared.
 Require Import LibFix LibList.
@@ -538,3 +540,4 @@ Proof.
 Qed.
 *)
 
+*)
